# Algebra

## Arithmetic operations

> Reference: @hass2018

* $a(b + c) = ab + ac$
* $\cfrac{a}{b} + \cfrac{c}{d} = \cfrac{ad + bc}{bd}$
* $\cfrac{a}{b} \times \cfrac{c}{d} = \cfrac{ac}{bd}$
* $\cfrac{a / b}{c / d} = \cfrac{a}{b} \times \cfrac{d}{c}$

## Laws of signs

> Reference: @hass2018

* $-(- a) = a$
* $\cfrac{-a}{b} = - \cfrac{a}{b} = \cfrac{a}{-b}$

## Zero

> Reference: @hass2018

Division by $0$ is not defined.

* $\text{If} \ \ \ a \ne 0: \cfrac{0}{a}$
* $a^{0} = 1$
* $0^{a} = 0$
* For any number $a$: $a \times 0 = 0 \times a = 0$

## Laws of expoents

> Reference: @hass2018

* $a^{m} a^{n} = a^{m + n}$
* $(ab)^{m} = a^{m} b^{m}$
* $(a^{m})^{n} = a^{mn}$
* $a^{m / n} = \sqrt[n]{a^{m}} = (\sqrt[n]{a})^{m}$

## The binominal theorem (Newton's binomial)

> Reference: @hass2018 and @khanacademy and @matika

For any positive integer $n$,

$$
(a + b)^{n} = a^{n} + na^{n - 1}b + \cfrac{n (n - 1)}{1 \cdot 2} a^{n - 2}b^{2} + \cfrac{n (n - 1) (n - 2)}{1 \cdot 2 \cdot 3}a^{n - 3}b^{3} + \cdots + nab^{n - 1} + b^{n}
$$

The same formula above can be written as

$$
(a + b)^{n} = \sum_{k = 0}^{n} \binom{n}{k} \cdot a^{n - k} \cdot b^{k} \quad , \quad \binom{n}{k} = \cfrac{n!}{k! (n - k)!}
$$

* Example:

$$
(a + b)^4 = a^{4} + 4a^{3}b + 6a^{2}b^{2} + 4ab^{3} + b^{4}
$$

In the case of $(a - b)$,

$$
(a - b)^{n} = \sum_{k = 0}^{n} \binom{n}{k} \cdot a^{n - k} \cdot (- b)^{k}
$$
Note that when the power of $âˆ’ b$ is even, the product is positive and if the power is odd, the product is negative.

* Example:

$$
(a - b)^4 = a^{4} - 4a^{3}b + 6a^{2}b^{2} - 4ab^{3} + b^{4}
$$

See the "special products" section for more examples.

## Pascal's triangle

> Reference: @wikiversity

![](../images/wikiversity_pascal-s-triangle_1.png)

![](../images/wikiversity_pascal-s-triangle_2.png)

![](../images/wikiversity_pascal-s-triangle_3.png)

## Factoring the difference of like integer powers, $n > 1$

> Reference: @hass2018

$$
a^{n} - b^{n} = (a - b)(a^{n - 1} + a^{n - 2}b + a^{n -3}b^{2} + \cdots + ab^{n - 2} + b^{n - 1})
$$

See the "special products" section for examples.

### Special products

> Reference: @hass2018

* Square of a sum: $(a + b)^{2} = a^{2} + 2ab + b^{2}$
* Square of a difference: $(a - b)^{2} = a^{2} - 2ab + b^{2}$
* Square of 3 terms sum: $(a + b + c)^{2} = a^{2} + b^{2} + c^{2} + 2ab + 2ac + 2bc$
* Cube of a sum: $(a + b)^3 = a^{3} + 3a^{2}b + 3ab^{2} + b^{3}$
* Cube of a difference: $(a - b)^{3} = a^{3} - 3a^{2}b + 3ab^{2} - b^{3}$
* Sum of cube: $a^{3} + b^{3} = (a + b)(a^{2} - ab + b^{2})$
* Difference of cube: $a^{3} - b^{3} = (a - b)(a^{2} + ab + b^{2})$
* Quad of a sum: $(a + b)^4 = a^{4} + 4a^{3}b + 6a^{2}b^{2} + 4ab^{3} + b^{4}$
* Quad of a difference: $(a - b)^4 = a^{4} - 4a^{3}b + 6a^{2}b^{2} - 4ab^{3} + b^{4}$
* Product of a sum: $(x + a)(x + b) = x^{2} + (a + b)x + ab$
* Product of a sum and a difference: $(a + b)(a - b) = a^{2} - b^{2}$

## Completing the square

> Reference: @hass2018

If $a \neq 0$, then

$$
ax^{2} + bx + c = au^{2} + C \quad \left (u = x + \cfrac{b}{2a} \ , \ C = c - \cfrac{b^2}{4a} \right )
$$

## The quadratic formula

> Reference: @hass2018

If $a \neq 0$ and $ax^{2} + bx + c = 0$, then

$$
x = \cfrac{-b \pm \sqrt{b^2 - 4ac}}{2a} \quad \left (\Delta = b^2 - 4ac  \right ) 
$$
