# Differential equations

## General differential equations

> Reference: @stewart2016b

In general, a __differential equation__ is an equation that contains an unknown function and one or more of its derivatives. The __order__ of a differential equation is the order of the highest derivative that occurs in the equation.

## Example of a differential equation: Population growth

> Reference: @stewart2016b

The rate of growth of the population is the derivative $\mathrm{d} P / \mathrm{d} t$, where $t = \text{time}$ (the independent variable) and $P = \text{the number of individuals in the population}$ (the dependent variable). So our assumption that the rate of growth of the population is proportional to the population size is written as the equation

$$
\cfrac{\mathrm{d} P}{\mathrm{d} t} = kP
$$

where $k$ is the proportionality constant. The equation above is a possible model for population growth; it is a differential equation because it contains an unknown function $P$ and its derivative $\mathrm{d} P / \mathrm{d} t$.

## Modeling with differential equations

> Reference: @stewart2016b

The mathematical model often takes the form of a differential equation. This is not surprising because in a real-world problem we often notice that changes occur and we want to predict future behavior on the basis of how current values change.

![The modeling process](../images/stewart_2016b_figure-1-2-1.png)

## Ordinary differential equations (Malthus’ model)

> Reference: @hase2022

Consider the Malthusian growth model,

$$
\cfrac{\mathrm{d}}{\mathrm{d} t} N(t) = \lambda N(t) \quad \lambda > 0
\tag{1}
$$

where $N(t)$ is the population at time $t$ and the initial condition (initial population) is $N(t = 0) = N_{0}$. In what follows, two possible resolutions will be presented.

### First resolution

In order to solve $(1)$, consider, __formally__, that the equation can be cast as

$$
\cfrac{\mathrm{d} N}{\mathrm{d} t} = \lambda N
$$

$$
\cfrac{\mathrm{d} N}{N} = \lambda \ \mathrm{d} t
$$

$$
\cfrac{1}{N} \mathrm{d} N = \lambda \ \mathrm{d} t
$$

$$
\int \cfrac{1}{N} \mathrm{d} N = \int \lambda \ \mathrm{d} t
,\quad \text{from which} \quad
\ln N = \lambda t + c',
\quad
c'\in \mathbb{R}
$$

In the equation above, two constants of integration are produced by the two integrals; the constant $c'$ above is the combination of both into a single one for simplicity. From it follows that

$$
\ln N = \lambda t + c'
$$

$$
e^{\ln N} = e^{\lambda t + c'}
$$

$$
N = e^{\lambda t + c'}, \quad (a^{\log_{a} x} = x)
$$

$$
N = e^{\lambda t} \cdot e^{c'}, \quad (a^{m} a^{n} = a^{m + n})
$$

$$
N(t) = c e^{\lambda t}, \quad (c = e^{c'})
$$

where $c = e^{c'}$; this constant is determined by the initial condition $N(0) = N_{0}$. For $t = 0$, one has

$$
N_{0} = N(0) = c e^{\lambda \cdot 0}, \quad \text{from which} \quad c = N_{0}
$$

hence,

$$
N(t) = N_{0} e^{\lambda t}
\tag{2}
$$

which is the solution of the problem.


### Second resolution

In order to solve $(1)$, consider, __formally__, that the equation can be cast as

$$
\cfrac{1}{N} \ \mathrm{d} N = \lambda \ \mathrm{d} t
$$

In this second resolution, one invokes the definite integrals; the integration runs from an initial configuration ($t = 0$ and $N(0) = N_{0}$) up to an arbitrary “final” situation ($t$ and $N(t)$): 

+:-------------:+:---:+:-------:+
| Variable      | $t$ | $N$     | 
+===============+=====+=========+
| Initial value | $0$ | $N_{0}$ |
+---------------+-----+---------+
| Final value   | $t$ | $N(t)$  |
+---------------+-----+---------+

Therefore, inserting the integration sign leads to

$$
\int^{N(t)}_{N_{0}} \cfrac{1}{N'} \ \mathrm{d} N' =
\int^{t}_{0} \lambda \ \mathrm{d} t'
$$

Note the relabeling $t'$ and $N'$ of the (dummy) variables of integration to avoid confusion with the integration limits. By evaluating the integrals of $(3)$, one achieves the solution $(2)$.

$$
\int^{N(t)}_{N_{0}} \cfrac{1}{N'} \ \mathrm{d} N' = \int^{t}_{0} \lambda \ \mathrm{d} t'
$$

$$
\biggr [ \ln N' \biggr ]^{N(t)}_{N_{0}} = \biggr [ \lambda t \biggr ]^{t}_{0}
$$

$$
\ln N(t) - \ln N_{0} = \lambda t - \lambda \cdot 0
$$

$$
\ln \left ( \cfrac{N(t)}{N_{0}} \right ) = \lambda t - \lambda \cdot 0, \quad \left( \log_{a} \left ( \cfrac{x}{y} \right ) = \log_{a} x - \log_{a} y \right )
$$

$$
e^{\ln \left ( \cfrac{N(t)}{N_{0}} \right )} = e^{\lambda t}
$$

$$
\cfrac{N(t)}{N_{0}} = e^{\lambda t}, \quad \left ( a^{\log_{a} x} = x \right )
$$
$$
N(t) = N_{0} e^{\lambda t}
$$

## Ordinary differential equations (Malthus-Verhulst’s model)

> Reference: @hase2022

Consider, now, the growth model of Malthus-Verhulst,

$$
\cfrac{\mathrm{d}}{\mathrm{d} t} N(t) = \lambda N(t) [C - N(t)]
, \quad
\lambda, C > 0
\tag{4}
$$

where $C$ (carrying capacity) is the maximum size of the population and the initial condition (population) is $N(t = 0) = N_{0}$. In order to solve $(4)$, one may write the equation __formally__, as

$$
\cfrac{\mathrm{d} N}{\mathrm{d} t} = \lambda N [C - N]
$$

$$
\lambda \ \mathrm{d} t = \cfrac{\mathrm{d} N}{N [C - N]}
$$
From

$$
\cfrac{1}{N [C - N]} = 
\cfrac{A}{N} + \cfrac{B}{[C - N]} = 
\cfrac{A [C - N] + BN}{N [C - N]} = 
\cfrac{AC - AN + BN}{N [C - N]} = 
\cfrac{N(B - A) + AC}{N [C - N]}
$$
One has,

$$
\begin{cases}
0 = B - A \\
1 = AC
\end{cases}
\quad , \quad \text{from which} \quad
\begin{cases}
A = \cfrac{1}{C} \\
B = \cfrac{1}{C}
\end{cases}
$$

Hence,

$$
\cfrac{1}{N [C - N]} = 
\cfrac{A}{N} + \cfrac{B}{[C - N]} = 
\cfrac{1}{C} \div N + \cfrac{1}{C} \div [C - N] =
\cfrac{1}{C} \cdot \cfrac{1}{N} + \cfrac{1}{C} \cdot \cfrac{1}{[C - N]}
$$

Then,

$$
\cfrac{1}{N [C - N]} \ \mathrm{d} N = 
\left [ \cfrac{1}{C} \cdot \cfrac{1}{N} + \cfrac{1}{C} \cdot \cfrac{1}{[C - N]} \right ]\ \mathrm{d} N
$$

$$
\cfrac{1}{N [C - N]} \ \mathrm{d} N = 
\cfrac{1}{C} \cdot \cfrac{\mathrm{d} N}{N} + \cfrac{1}{C} \cdot \cfrac{\mathrm{d} N}{[C - N]}
$$

Going back to the original equation, we then have,

$$
\lambda \ \mathrm{d} t = \cfrac{1}{C} \cdot \cfrac{\mathrm{d} N}{N} + \cfrac{1}{C} \cdot \cfrac{\mathrm{d} N}{C - N}
$$

In what follows, two possible resolutions will be presented.

### First resolution

In order to solve $(4)$, consider, __formally__, that the equation can be cast as

$$
\lambda \ \mathrm{d} t = \cfrac{1}{C} \cdot \cfrac{\mathrm{d} N}{N} + \cfrac{1}{C} \cdot \cfrac{\mathrm{d} N}{C - N}
$$
$$
\int \lambda \ \mathrm{d} t = \int \left [ \cfrac{1}{C} \cdot \cfrac{1}{N} + \cfrac{1}{C} \cdot \cfrac{1}{C - N} \right ] \ \mathrm{d} N
$$

$$
\int \lambda \ \mathrm{d} t = \int \left [ \cfrac{1}{C} \cdot \cfrac{1}{N} \right ] \ \mathrm{d} N + \int \left [ \cfrac{1}{C} \cdot \cfrac{1}{C - N} \right ] \ \mathrm{d} N
$$

$$
\int \lambda \ \mathrm{d} t = \cfrac{1}{C} \int \cfrac{1}{N} \ \mathrm{d} N + \cfrac{1}{C} \int \cfrac{1}{C - N} \ \mathrm{d} N
$$

Where,

$$
u = C - N, \quad \cfrac{\mathrm{d} u}{\mathrm{d} N} = -1, \quad \mathrm{d} N = - \mathrm{d} u
$$

$$
- \int \cfrac{1}{u} \ \mathrm{d} u = - \ln |u| + c = - \ln |C - N| + c
$$

From which

$$
\lambda t = \cfrac{1}{C} \ln |N| - \cfrac{1}{C} \ln |C - N| + c'
$$
The constant $c′$ above is the combination of all $c$ into a single one for simplicity.

$$
\lambda t = \cfrac{1}{C} [ \ln |N| - \ln |C - N| ] + c'
$$

$$
\lambda t = \cfrac{1}{C} \ln \left ( \cfrac{|N|}{|C - N|} \right ) + c'
, \quad \left ( \log_{a} \left ( \cfrac{x}{y} \right ) = \log_{a} x - \log_{a} y \right )
$$

$$
\lambda t = \cfrac{1}{C} \ln \left | \cfrac{N}{C - N} \right | + c'
$$

since $0 \leq N(t) \leq C$

$$
\lambda t = \cfrac{1}{C} \ln \left ( \cfrac{N}{C - N} \right ) + c'
, \quad (c' \in \mathbb{R})
$$

In similar way made with the Malthus’ model, the formula above can be cast as

$$
N(t) = \cfrac{C}{1 + k e^{- \lambda C t}}
$$

where $k = e^{c'}$; this constant is determined by the initial condition $N(0) = N_{0}$. For $t = 0$, one has

$$
N_{0} = N(0) = \cfrac{C}{1 + k}
$$

From which

$$
k = \cfrac{C}{N_{0}} - 1
$$

Hence,

$$
N(t) = \cfrac{C N_{0}}{N_{0} + (C - N_{0}) e^{- \lambda C t}}\
\tag{3}
$$

which is the solution of the problem.

### Second resolution

In this second resolution, one invokes the definite integrals; the integration runs from an initial configuration ($t = 0$ and $N(0) = N_{0}$) up to an arbitrary “final” situation ($t$ and $N(t)$): 

+:-------------:+:---:+:-------:+
| Variable      | $t$ | $N$     | 
+===============+=====+=========+
| Initial value | $0$ | $N_{0}$ |
+---------------+-----+---------+
| Final value   | $t$ | $N(t)$  |
+---------------+-----+---------+

Therefore, inserting the integration sign leads to

$$
\lambda \ \mathrm{d} t = \cfrac{1}{C} \cdot \cfrac{\mathrm{d} N}{N} + \cfrac{1}{C} \cdot \cfrac{\mathrm{d} N}{C - N}
$$

$$
\lambda \ \mathrm{d} t = \cfrac{1}{C} \left ( \cfrac{1}{N} + \cfrac{1}{C - N} \right ) \ \mathrm{d} N
$$

$$
\int^{N(t)}_{N_{0}} \cfrac{1}{C} \left ( \cfrac{1}{N'} + \cfrac{1}{C - N'} \right ) \ \mathrm{d} N' = \int^{t}_{0} \lambda \ \mathrm{d} t'
$$

$$
\cfrac{1}{C} \int^{N(t)}_{N_{0}} \left ( \cfrac{1}{N'} + \cfrac{1}{C - N'} \right ) \ \mathrm{d} N' = \int^{t}_{0} \lambda \ \mathrm{d} t'
$$

Note the relabeling $t'$ and $N'$ of the (dummy) variables of integration to avoid confusion with the integration limits. By evaluating the integrals above, one achieves the solution $(3)$.

## Examples

> Reference: @hase2022

### Example 1

$$
\cfrac{\mathrm{d}}{\mathrm{d} x} y = x, \quad y(x_{0}) = y_{0}
$$

From

$$
\mathrm{d} y = x \mathrm{d} x
$$

$$
\int \mathrm{d} y = \int x \ \mathrm{d} x
$$

$$
y = \cfrac{x^{2}}{2} + c, \quad (c \in \mathbb{R})
$$

From the condition $y(x_{0}) = y_{0}$, one has

$$
y_{0} = \cfrac{x^{2}_{0}}{2} + c
$$

From which

$$
c = y_{0} - \cfrac{x^{2}_{0}}{2}
$$

Then,

$$
y = \cfrac{x^{2}}{2} + y_{0} - \cfrac{x^{2}_{0}}{2}
$$

### Example 2

$$
\cfrac{\mathrm{d}}{\mathrm{d} x} y = \cfrac{x}{y}, \quad y(0) = 2
$$

From

$$
y \ \mathrm{d} y = x \ \mathrm{d} x
$$

$$
\int^{y}_{2} y' \ \mathrm{d} y' = \int^{x}_{0} x' \ \mathrm{d} x' 
$$

one has

$$
\biggr [ \cfrac{y'^{2}}{2} \biggr ]^{y}_{2} = \biggr [ \cfrac{x'^{2}}{2} \biggr ]^{x}_{0}
$$

$$
\cfrac{y^{2}}{2} - \cfrac{2^{2}}{2} = \cfrac{x^{2}}{2} - \cfrac{0^{2}}{2}
$$
$$
\cfrac{y^{2} - 4}{2} = \cfrac{x^{2}}{2}
$$

$$
y^{2} - 4 = x^{2}
$$

$$
y^{2} = x^{2} + 4
$$

$$
y(x) = \pm \sqrt{x^{2} + 4}
$$

### Important example 

$$
\cfrac{\mathrm{d}}{\mathrm{d} t} y = a y + b, \quad a, b \in \mathbb{R}
$$

From

$$
\cfrac{\mathrm{d} y}{a y + b} = \mathrm{d} t
$$

$$
\int \cfrac{1}{a y + b} \ \mathrm{d} y = \int \mathrm{d} t
$$

One has

$$
\cfrac{1}{a} \ln |ay + b| = t + c_{1}
\quad \text{or} \quad
\ln |ay + b| = at + c_{2}
\quad c_{1} \in \mathbb{R}
\quad c_{2} = a c_{1} \in \mathbb{R}
\tag{4}
$$

Then,

$$
e^{\ln |ay + b|} = e^{at + c_{2}}
$$

$$
|ay + b| = e^{at + c_{2}}, \quad (a^{\log_{a} x} = x)
$$

$$
|ay + b| = e^{at} e^{c_{2}}, \quad (a^{m} a^{n} = a^{m + n})
$$

$$
|ay + b| = c_{3} e^{at}
$$

where $c_{3} = e^{c_{2}} = e^{a c_{1}}$ is now a __positive__ real number.

From the modulus sign, one has

$$
ay + b = \pm c_{3} e^{at}
$$

Incorporating the sign into the constant term leads to

$$
ay + b = K e^{at}
$$

where now $K \in \mathbb{R} ∖ \{0\}$. Therefore,

$$
y(t) = \cfrac{K e^{at} - b}{a}
$$

and $K$ is a nonzero constant. This condition is satisfied, since $K = 0$ requires the integration constant $c_{1}$ to diverge ($c_{1} \to \infty$ if $a < 0$, and $c_{1} \to - \infty$ if $a > 0$). It is curious to realize that the same solution above is obtained if one performs the calculation “ignoring” the modulus sign of the argument of logarithm in $(4)$.
