# Integrals

## Antiderivatives and indefinite integrals

> Reference: @hase2022

The derivative $f'$ of a function $f : \mathbb{R} \to \mathbb{R}$ is defined by the formula

$$
f'(x) = \lim \limits_{\Delta x \to 0} = \cfrac{f(x + \Delta x) - f(x)}{\Delta x}
$$

Now, a different question can be proposed: given $f$, one may be interested in a function $F$ such that

$$
F'(x) = f(x)
$$

for all $x$ in the domain of $f$. This is an inverse problem of derivation, and $F$ is called an __antiderivative__ of $f$. One may immediately note that the antiderivative of a function is not unique; for instance, if $f(x) = x$, then $\cfrac{x^{2}}{2}$, $\cfrac{x^{2}}{2} − 1$ and $\cfrac{x^{2}}{2} + \pi$ are some possible antiderivatives. However, as these examples indicate, the difference between any two antiderivatives of a given function is a constant. This means that if $F$ is an antiderivative of $f$, any other antiderivative of $f$ can be expressed by $F + c$, where $c \in \mathbb{R}$ is a constant.

If $F(x)$ is an antiderivative of $f(x)$ for $x \in (a, b) \subset \mathbb{R}$, the __family of functions__ $\{F + c\}$, where $c \in \mathbb{R}$ is a constant, is the __indefinite integral__ of $f$, and is denoted by

$$
\int f(x) \ dx
$$

_id est_,

$$
\int f(x) \ \mathrm{d} x = F(x) + c, \quad c \in \mathbb{R}, \quad \text{if} \quad F'(x) = f(x)
$$

In $\displaystyle \int f(x) \ dx$, $f(x)$ is the integrand and the symbol $dx$ (the measure of integration) will play an important role later. Some remarks: 

1. From the definition, $\displaystyle \cfrac{\mathrm{d}}{\mathrm{d} x} \int f(x) \ \mathrm{d} x = f(x)$.

2. Geometrically, an indefinite integral is a family of curves, each one of them being related to others by a “vertical” translation.

3. Not every function has an indefinite integral; furthermore, not every function has an indefinite integral that can be expressed by a finite combination of elementary functions.

Indefinite integrals are also defined for linear combinations of functions. As a consequence of linearity in derivatives, the following linear properties hold:

* $\displaystyle \int [f(x) + f(x)] \ \mathrm{d} x = \int f(x) \ \mathrm{d} x + \int g(x) \ \mathrm{d} x$
* $\displaystyle \int \alpha f(x) \ \mathrm{d} x = \alpha \int f(x) \ \mathrm{d} x \quad (\alpha \in \mathbb{R})$

To see the properties above, one should derive both sides of each identity and see that the results match. The identities should be understood in the sense that indefinite integrals are __equivalent up to a constant__. In particular, it
follows that

$$
0 \cdot \int f(x) \ \mathrm{d} x = \int 0 \cdot f(x) \ \mathrm{d} x = \int 0 \ \mathrm{d} x = c \quad (c \in \mathbb{R})
$$

and

$$
\int f(x) \ \mathrm{d} x - \int f(x) \ \mathrm{d} x = \int [f(x) - f(x)] \ \mathrm{d} x = \int 0 \ \mathrm{d} x = c \quad (c \in \mathbb{R})
$$

These two examples remind one that indefinite integrals are a family of functions, and not simple functions.

## Indefinite integrals of elementary functions

> Reference: @hase2022 and @morettin2003

For all $c \in \mathbb{R}$:

* $\displaystyle \int \cos x \ \mathrm{d} x = \sin x + c \quad , \quad \text{since} \ \ \cfrac{\mathrm{d}}{\mathrm{d} x} \sin x = \cos x$
* $\displaystyle \int \sin x \ \mathrm{d} x = - \cos x + c \quad , \quad \text{since} \ \ \cfrac{\mathrm{d}}{\mathrm{d} x} ( - \cos x) = \sin x$
* $\displaystyle \int \sec^{2} x \ \mathrm{d} x = \tan x + c \quad , \quad \text{since} \ \ \cfrac{\mathrm{d}}{\mathrm{d} x} \tan x = \sec^{2} x$
* $\displaystyle \int e^{2} \ \mathrm{d} x = e^{2} + c \quad , \quad \text{since} \ \ \cfrac{\mathrm{d}}{\mathrm{d} x} e^{2} = e^{2}$

* $\displaystyle \int \alpha x^{\alpha - 1} \ \mathrm{d} x = x^{\alpha} + c \quad , \quad \text{since} \ \ \cfrac{\mathrm{d}}{\mathrm{d} x} x^{\alpha} = \alpha x^{\alpha - 1}$
  
  * $\displaystyle \int x^{\alpha} \ \mathrm{d} x = \cfrac {x^{\alpha + 1}} {\alpha + 1} + c \quad (\alpha \neq -1)$ 

* $\displaystyle \int \cfrac{1}{x} \ \mathrm{d} x = \ln |x| + c \quad , \quad \text{since} \ \ \cfrac{\mathrm{d}}{\mathrm{d} x} \ln |x| = \cfrac{1}{x}$

## (Riemann) Integral - Definition

> Reference: @hase2022

Let $f : \mathbb{R} \to \mathbb{R}$ be a continuous function. Considering an interval $[a, b] \subset \mathbb{R}$, it is possible to choose a partition given by $a = x_{0} < x_{1} < \cdots  < x_{N - 1} < x_{N} = b$ (figure 1) from which one can define the sum

$$
\sum \limits^{N}_{n = 1}  f(x_{n}) \Delta x_{n} \quad \text{where} \quad \Delta x_{n} := x_{n} - x_{n - 1}
$$

Note that if $f \geq 0$ in $[a, b]$, this sum approaches the area between $f$ and the $x$ axis when 

$\text{(a)}$ The size of each division is diminished.

$\text{(b)}$ The number of divisions inside the partition is increased.

![Figure 1: Decomposition in rectangles](../images/hase_lecture_7_figure_1.png)

It should be clear that $\text{(a)}$ implies $\text{(b)}$, but the converse is false. The limit of such sum is the (Riemann) integral of $f$ in the interval $[a, b]$, and is denoted by

$$
\int^{b}_{a} f(x) \ \mathrm{d} x := \lim \limits_{\text{max}_{n} \ \Delta x_{n} \to 0} \sum \limits^{N}_{n = 1}  f(x_{n}) \Delta x_{n}
$$

The interpretation of the formula above as being the area becomes clearer if the quantity $\displaystyle \int^{b}_{a} f(x) \ \mathrm{d} x$ is understood as $\displaystyle \int^{b}_{a} [f(x) - 0] \ \mathrm{d} x$. Hence, if $f \leq 0$ at $[a, b]$, $\displaystyle \int^{b}_{a} f(x) \ \mathrm{d} x$ would be the “opposite of the area”. The continuity condition of $f$ can be relaxed to piecewise continuity.

Two properties of the definite integral are assumed by definition:

$$
\int^{b}_{a} f(x) \ \mathrm{d} x = - \int^{a}_{b} f(x) \ \mathrm{d} x
\tag{i}
$$

$$
\int^{a}_{a} f(x) \ \mathrm{d} x = 0
\tag{ii}
$$

## General formulas

> Reference: @hass2018

* Zero: $\displaystyle \int^{a}_{a} f(x) \ \mathrm{d} x = 0$
* Order of integration: $\displaystyle \int^{a}_{b} f(x) \ \mathrm{d} x = - \int^{b}_{a} f(x) \ \mathrm{d} x$

* Constant multiples:

  * $\displaystyle \int^{b}_{a} k f(x) \ \mathrm{d} x = k \int^{b}_{a} f(x) \ \mathrm{d} x, \quad k \in \mathbb{R}$
  * $\displaystyle \int^{b}_{a} - f(x) \ \mathrm{d} x = - \int^{b}_{a} f(x) \ \mathrm{d} x, \quad k = -1$

* Sum: $\displaystyle \int^{b}_{a} [(f(x) + g(x)] \ \mathrm{d} x = \int^{b}_{a} f(x) \ \mathrm{d} x + \int^{b}_{a} g(x) \ \mathrm{d} x$
* Difference: $\displaystyle \int^{b}_{a} [(f(x) - g(x)] \ \mathrm{d} x = \int^{b}_{a} f(x) \ \mathrm{d} x - \int^{b}_{a} g(x) \ \mathrm{d} x$
* Additivity: $\displaystyle \int^{b}_{a} f(x) \ \mathrm{d} x + \int \limits^{c}_{b} f(x) \ \mathrm{d} x = \int \limits^{c}_{a} f(x) \ \mathrm{d} x$
* Max-min inequality: If max $f$ and min $f$ are the maximum and minimum values of $f$ on $[a, b]$, then

$$
\text{min} \ f \cdot (b - a) \leq \int^{b}_{a} f(x) \ \mathrm{d} x \leq \text{max} \ f \cdot (b - a)
$$

* Domination:

  * $\displaystyle f(x) \geq g(x) \quad \text{on} \quad [a, b] \quad \text{implies} \quad \int^{b}_{a} f(x) \ \mathrm{d} x \geq \int^{b}_{a} g(x) \ \mathrm{d} x$
  * $\displaystyle f(x) \geq 0 \quad \text{on} \quad [a, b] \quad \text{implies} \quad \int^{b}_{a} f(x) \ \mathrm{d} x \geq 0$

## (Riemann) Integral - Fundamental theorem of calculus

> Reference: @hase2022

This section establishes a connection between the integral of a function and its derivative. Concretely, this connection allows one to evaluate some integrals in terms of some known functions.

Let $f$ be continuous in $\mathbb{R}$ (for simplicity) and consider the function

$$
F(x) := \int^{x}_{a} f(\xi) \ \mathrm{d} \xi
\tag{iii}
$$

which represents the integral of $f$ from point $a$ (fixed) to another point $x$ (variable). Then, from the properties shown in the section above, it follow that

$$
\cfrac{F(x + \Delta x) - F(x)}{\Delta x} = 
\cfrac{1}{\Delta x} \left [ \int^{x + \Delta x}_{a} f(\xi) \ \mathrm{d} \xi - \int^{x}_{a} f(\xi) \ \mathrm{d} \xi \right ] = 
\cfrac{1}{\Delta x} \int^{x + \Delta x}_{x} f(\xi) \ \mathrm{d} \xi
$$

The integral above is evaluated in the interval $[x, x + \Delta x)$; if the value of $\Delta x \ (> 0)$ is decreased, one has $f(\xi) \approx f(x)$ for $\xi \in [x, x + \Delta x)$, since $f$ is continuous. Therefore, 

$$
\cfrac{\mathrm{d}}{\mathrm{d} x} F(x) = 
\lim \limits_{\Delta x \to 0} \cfrac{F(x + \Delta x) - F(x)}{\Delta x} = 
\lim \limits_{\Delta x \to 0} \cfrac{1}{\Delta x} \int^{x + \Delta x}_{a} \underbrace{f(\xi)}_{\simeq f(x)} \ \mathrm{d} \xi = 
$$

$$
= \lim \limits_{\Delta x \to 0} \cfrac{1}{\Delta x} f(x) \int^{x + \Delta x}_{a}  \mathrm{d} x = f(x) 
$$

remembering that the integral (in the variable $\xi$) does not act over $f(x)$, which is considered to be “constant”; moreover, $\displaystyle \int^{x + \Delta x}_{a}  \mathrm{d} \xi = \int^{x + \Delta x}_{a} 1 \ \mathrm{d} \xi$ is the area of the rectangle defined between the constant function $1$ and the $x$-axis in the interval $\xi \in [x, x + \Delta x)$. As a consequence, one has 

$$
\cfrac{\mathrm{d}}{\mathrm{d} x} \int^{x}_{a} f(\xi) \ \mathrm{d} \xi = f(x)
\tag{iv}
$$

Note that this result does not depend on the choice of $a$.

Suppose, now, that there is a function $g$ such that $f = g'$. This means that both $F$ and $g$ are antiderivatives of $f$. From $\text{(iii)}$ and $\text{(iv)}$, one has $F' = f = g'$ and, from the linearity of derivatives, $(F − g)' = 0$. Hence, the function $F − g$ should equal a constant, $c \in \mathbb{R}$, from which

$$
F(x) = g(x) + c \quad (x \in \mathbb{R})
$$

Since $F(a) = 0$ by $\text{(iii)}$, it is straightforward that $c = − g(a)$; then, $F(x) = g(x) − g(a)$ by the formula above. Finally, by choosing $x = b$ in $\text{(iii)}$, which implies $F(b) = g(b) − b(a)$, one has

$$
\int^{b}_{a} f(x) \ \mathrm{d} x = g(b) - g(a), \quad \text{where} \quad f = g'
$$

This is the definite integral, which is a “number”(indefinite integrals are families of functions). To evaluate the integral of $f$ from $a$ to $b$, it is necessary, then, to find a function $g$ whose derivative is $f$ and compute the difference $g(b) − g(a)$. Finally, one also has

$$
\int^{b}_{a} \left [ \cfrac{\mathrm{d}}{\mathrm{d} x} f(x) \right ] \ \mathrm{d} x = \int^{b}_{a} f'(x) \ \mathrm{d} x = f(b) - f(a)
$$

since $f$ is a function whose derivative is $f'$.

__Example__: $\displaystyle \int^{\pi}_{0} \sin x \ \mathrm{d} x$

Firstly,

$$
\int^{\pi}_{0} \sin x \ \mathrm{d} x = F(\pi) - F(0)
$$

where $F$ is such that $F' = f$. Therefore, taking $F(x) = − \cos x$ is a possibility (actually $\cos x + c$, $c \in \mathbb{R}$, also works, but the constant $c$ plays no role, since it cancels out in the difference $F(\pi) - F(0)$); as a consequence,

$$
\int^{\pi}_{0} \sin x \ \mathrm{d} x = [- \cos \pi] - [- \cos 0] = 2
$$

__Example__: $\displaystyle \int^{3}_{1} \left ( \cfrac{x^{3} - x}{x} \right ) \ \mathrm{d} x$

Since $\cfrac{x^{3} - x}{x} = \cfrac{x^{3}}{x} - \cfrac{x}{x} = x^{2} - 1$ (for $x \neq 0$), then,

$$
\int^{3}_{1} \left ( \cfrac{x^{3} - x}{x} \right ) \ \mathrm{d} x = 
\int^{3}_{1} x^{2} \ \mathrm{d} x - \int^{3}_{1} 1 \ \mathrm{d} x = 
$$

$$
= \biggr [ \underbrace{\cfrac{x^{3}}{3}}_{\text{antiderivative of} \ x^{2}} \biggr ]^{3}_{1} - \biggr [ \underbrace{x}_{\text{antiderivative of} \ 1} \biggr ]^{3}_{1} = 
\biggr [ \cfrac{3^{3}}{3} - \cfrac{1^{3}}{3} \biggr ] - \biggr [ 3 - 1 \biggr ] = \cfrac{20}{3}
$$
