# Limits

## Continuity

> Reference: @hase2022

If $P(x)$ is continuous at $x = c$, i.e., $\lim \limits_{x \to c^{-}} f(x) = \lim \limits_{x \to c^{+}} f(x)$, then 

$$\lim \limits_{x \to c} f(x) = f(c)$$

## Inequalities

> Reference: @hass2018

If $f(x) \leq g(x)$ in an open interval containing $c$, except possibly at $x = c$, and both limits exists, then:

$$\lim \limits_{x \to c} f(x) \leq \lim \limits_{x \to c} g(x)$$

## General laws

> Reference: @hass2018

If $L$, $M$, $c$, and $k$ are real numbers and

$\lim \limits_{x \to c} f(x) = L$ and $\lim \limits_{x \to c} g(x) = M$, then

* Sum rule: $\lim \limits_{x \to c} [f(x) + g(x)] = L + M = \lim \limits_{x \to c} f(x) + \lim \limits_{x \to c} g(x)$

    Example: $\lim \limits_{x \to 1} [x^{2} + 3x^{3}] = \lim \limits_{x \to 1} x^{2} + \lim \limits_{x \to 1} 3x^{3} = 1 + 3 = 4$

* Difference rule: $\lim \limits_{x \to c} [f(x) - g(x)] = L - M = \lim \limits_{x \to c} f(x) - \lim \limits_{x \to c} g(x)$

* Product rule: $\lim \limits_{x \to c} [f(x) \times g(x)] = L \times M = \lim \limits_{x \to c} f(x) \times \lim \limits_{x \to c} g(x)$

* Constant multiple rule: $\lim \limits_{x \to c} (k \times f(x)) = k \times L = k \times \lim \limits_{x \to c} f(x)$

* Quotient rule: $\lim \limits_{x \to c} \cfrac{f(x)}{g(x)} = \cfrac{L}{M} = \cfrac{\lim \limits_{x \to c} f(x)}{\lim \limits_{x \to c} g(x)}$, $M \neq 0$, $\lim \limits_{x \to c} g(x) \neq 0$

## Infinite limit of rational functions

> Reference: @hase2022

$$\lim \limits_{x \pm \infty} \cfrac{P_{n}(x)}{Q_{m}(x)} = \lim \limits_{x \pm \infty} \cfrac{a_{n}x^{n} + a_{n - 1}x^{n - 1} \cdots + a_{1}x + a_{0}}{b_{m}x^{m} + b_{m - 1}x^{m - 1} \cdots + b_{1}x + b_{0}} = \lim \limits_{x \pm \infty} \cfrac{x^{n} (a_{n} + \frac{a_{n - 1}}{x} \cdots + \frac{a_{1}}{x^{n - 1}} + \frac{a_{0}}{x^{n}})}{x^{m} (b_{m} + \frac{b_{m - 1}}{x} \cdots + \frac{b_{1}}{x^{m - 1}} + \frac{b_{0}}{x^{m}})}$$


* $n = m$: in this case, the largest term of the numerator ($a_{n}x^{n}$) is of the same order of magnitude with the largest term of the denominator ($b_{m}x^{m} = b_{n}x^{n}$), and the limit converges to $\cfrac{a_{n}}{b_n}$.

* $n < m$: n this case, the denominator is much larger than the numerator, and the limit converges to zero.

* $n > m$: in this case, one should analyze the sign of the dominant term of the limit, which is $\cfrac{a_{n}}{b_m} x^{n - m}$. If $\cfrac{a_{n}}{b_m} x^{n - m} > 0$ when $x \to \pm \infty$, then $\lim \limits_{x \pm \infty} \cfrac{P_{n}(x)}{Q_{m}(x)} \to \infty$. On the other hand, if $\cfrac{a_{n}}{b_m} x^{n - m} < 0$, when $x \to \pm \infty$, then $\lim \limits_{x \pm \infty} \cfrac{P_{n}(x)}{Q_{m}(x)} \to - \infty$

## Squeeze theorem (or sandwich theorem)

> Reference: @hase2022

For an interval $I \subset \mathbb{R}$, assume that $g(x) \leq f(x) \leq h(x)$ with $x \in I$. Given $x_{0} \in I$, if

$$\lim \limits_{x \to x_{0}} g(x) = \lim \limits_{x \to x_{0}} h(x) = L \ \text{, then} \ \lim \limits_{x \to x_{0}} f(x) = L$$.

![](../images/hase_lecture_1_figure_3.png)

## The fundamental limit

> Reference: @hase2022

![](../images/hase_lecture_1_figure_4.png)

Denote by $S_{\triangle OPQ}$, $S_{\triangle OPR}$, and $S_{\sector OPQ}$, respectively, the areas of the triangles $OPQ$, $OPR$ and the circular section $OPQ$, as in figure 4. Let $r$ be the radius of the disk. It is straightforward that

$$S_{\triangle OPQ} \leq S_{\sector OPQ} \leq S_{\triangle OPR}$$

Since $S_{\triangle OPQ} = \cfrac{r^{2} \sin x}{2}$, $S_{\sector OPQ} = \cfrac{r^{2} x}{2}$, and $S_{\triangle OPR} = \cfrac{r^{2} \tan x}{2}$, the above inequality implies

$$\sin x \leq x \leq \tan x \ \ \ \ \ \text{or} \ \ \ \ \ \cos x \leq \cfrac{\sin x}{x} \leq 1$$

Therefore, since $\lim \limits_{x \to 0} \cos x = 1$ from the squeeze theorem, it follows that

$$\lim \limits_{x \to 0} \cfrac{\sin x}{x} = 1$$

One should be aware that __this fundamental limit is valid when the angle $x$ is measured in radians__. If $x$ is measured in degree, one would have $S_{\sector OPQ} = \cfrac{r^{2} x}{2} \cfrac{\pi}{180}$, which would have lead to $\lim \limits_{x \to 0} \cfrac{\sin x}{x} = \cfrac{\pi}{180}$.

## Special formulas

> Reference: @hase2022

* If $P(x) = a_{n}x^{n} + a_{n - 1}x^{n - 1} + \cdots + a_{0}$, then $\lim \limits_{x \to c} P(x) = P(c) = a_{n}c^{n} + a_{n - 1}c^{n - 1} + \cdots + a_{0}$

* If $P(x)$ and $Q(x)$ are polynomials and $Q(c) \neq 0$, then $\lim \limits_{x \to c} \cfrac{P(x)}{Q(x)} = \cfrac{P(c)}{Q(c)}$

* If $f(x)$ is continuous at $x = c$, then $\lim \limits_{x \to c} f(x) = f(c)$ , $\lim \limits_{x \to c} \cfrac{\sin x}{x} = 1$ , and $\lim \limits_{x \to c} \cfrac{1 - \cos x}{x} = 0$

## Other properties

> Reference: @morettin2003 | @somatematica | @ventura

* $\lim \limits_{x \to \pi} [3x^{3} \times \cos x] = \lim \limits_{x \to \pi} 3x^{3} \times \lim \limits_{x \to \pi} \cos x = 3\pi ^{3} \times cos \pi = 3 \pi ^{3} \times (-1) = - 3 \pi ^{3}$

* $\lim \limits_{x \to \pi} [3x^{3} \times \cos x] = \lim \limits_{x \to \pi} 3x^{3} \times \lim \limits_{x \to \pi} \cos x = 3\pi ^{3} \times cos \pi = 3 \pi ^{3} \times (-1) = - 3 \pi ^{3}$

    Example: $\lim \limits_{x \to 0} \cfrac{\cos x}{x^{2} + 1} = \cfrac{\lim \limits_{x \to 0} \cos x}{\lim \limits_{x \to 0} x^{2} + 1} = \cfrac{\cos 0}{0^{2} + 1} = \cfrac{1}{1} = 1$

* $\lim \limits_{x \to a} f(x)^{n} = \left( \lim \limits_{x \to a} f(x) \right) ^{n}$, desde que $n \in \mathbb{N}^{*}$

    Example: $\lim \limits_{x \to 1} (x^{2} + 3)^{2} = \left[ \lim \limits_{x \to 1} (x^{2} + 3)^{2} \right] = (1 + 3)^{2} = 16$

* $\lim \limits_{x \to a} \sqrt[n]{f(x)} = \sqrt[n]{\lim \limits_{x \to a} f(x)}$, desde que $n \in \mathbb{N}^{*}$ e $f(x) > 0$ (se $f(x) \leq 0$ $n$ é ímpar)

* $\lim \limits_{x \to 2} \sqrt{x^{3} + x^{2} - 1} = \sqrt{\lim \limits_{x \to 2} x^{3} + x^{2} - 1} = \sqrt{2^{3} + 2^{2} - 1} = \sqrt{11}$

* $\lim \limits_{x \to a} (\ln f(x)) = \ln \left[ \lim \limits_{x \to a} f(x) \right]$, desde que $\lim \limits_{x \to a} f(x) > 0$

    Example: $\lim \limits_{x \to e} (\ln x^{2}) = \ln \left[ \lim \limits_{x \to e} x^{2} \right] = \ln e^{2} = 2 \ln e = 2 \times 1 = 2$

* $\lim \limits_{x \to a} \sin (f(x)) = \sin \left( \lim \limits_{x \to a} f(x) \right)$

    Example: $\lim \limits_{x \to 1} \sin (x^{2} + 3x) = \sin \left[ \lim \limits_{x \to 1} (x^{2} +3x) \right] = \sin 4$

* $\lim \limits_{x \to a} e^{f(x)} = e^{\lim \limits_{x \to a} f(x)}$

    Example: $\lim \limits_{x \to 1} e^{x^{2} + 3x} = e^{\lim \limits_{x \to 1} x^{2} +3x} = e^{4}$

## The l'Hôpital's rule

> Reference: @hase2022

Theorem: Let $f$ and $g$ be two differentiable functions on an open interval $I$ and let $\lim \limits_{x \to a} f(x) = \lim \limits_{x \to a} g(x) = \pm \infty$ or $0$ (here, $a \in \mathbb{R} \cup \{+ \infty, -\infty\}$, and $f$ and $g$ need not be defined on $a$). Furthermore, if $g′(x) \ne 0$ at $I ∖ \{a\}$ and $\lim \limits_{x \to a} \cfrac{f′(x)}{g′(x)}$ exists, then

$$\lim \limits_{x \to a} \cfrac{f(x)}{g(x)} = \lim \limits_{x \to a} \cfrac{f′(x)}{g′(x)}$$
